Path.dfy
@@ -1,0 +1,622 @@
+module Path {
+
+  import opened Circ
+  import opened Eval
+  import opened MapFunction
+  import opened Utils
+
+  function PathSegment(p: seq<NP>, start: nat, stop: nat): (seg: seq<NP>)
+    requires start < |p|
+    requires stop <= |p|
+    requires start < stop
+    ensures |p| > 0
+  {
+    p[start..stop]
+  }
+
+  lemma PathSegmentValid(c: Circuit, p: seq<NP>, start: nat, stop: nat)
+    requires c.Valid()
+    requires PathValid(c, p)
+    requires start < |p|
+    requires stop <= |p|
+    requires start < stop
+    ensures
+      var p := PathSegment(p, start, stop);
+      PathValid(c, p)
+  {
+    reveal PathValid();
+  }
+
+  function ValidPathSegment(c: Circuit, p: seq<NP>, start: nat, stop: nat): (seg: seq<NP>)
+    requires c.Valid()
+    requires PathValid(c, p)
+    requires start < |p|
+    requires stop <= |p|
+    requires start < stop
+    ensures
+      PathValid(c, seg)
+  {
+    PathSegmentValid(c, p, start, stop);
+    PathSegment(p, start, stop)
+  }
+
+  ghost opaque predicate PathExists(c: Circuit, np_a: NP, np_b: NP)
+    requires c.Valid()
+  {
+    exists p: seq<NP> :: (|p| > 0) && PathValid(c, p) && (Seq.First(p) == np_a) && (Seq.Last(p) == np_b)
+  }
+
+  ghost function PathExistsToPath(c: Circuit, np_a: NP, np_b: NP): (path: seq<NP>)
+    requires c.Valid()
+    requires PathExists(c, np_a, np_b)
+  {
+    reveal PathExists();
+    var path :| (|path| > 0) && PathValid(c, path) && (Seq.First(path) == np_a) && (Seq.Last(path) == np_b);
+    path
+  }
+
+  predicate PathToNPSet(c: Circuit, p: seq<NP>, np: NP, nps_b: set<NP>)
+    requires c.Valid()
+  {
+    (|p| > 0) && PathValid(c, p) && (Seq.First(p) == np) && (Seq.Last(p) in nps_b)
+  }
+
+  opaque ghost predicate PathExistsToNPSet(c: Circuit, np: NP, nps_b: set<NP>)
+    requires c.Valid()
+  {
+    exists p: seq<NP> :: PathToNPSet(c, p, np, nps_b)
+  }
+
+  lemma StillNoPathExistsToNPSet(c: Circuit, np: NP, next_np: NP, nps_b: set<NP>)
+    requires c.Valid()
+    requires NPValid(c, np)
+    requires NPValid(c, next_np)
+    requires NPsConnected(c, np, next_np)
+    requires !PathExistsToNPSet(c, np, nps_b)
+    ensures !PathExistsToNPSet(c, next_np, nps_b)
+  {
+    reveal PathExistsToNPSet();
+    if PathExistsToNPSet(c, next_np, nps_b) {
+      var p :| (|p| > 0) && PathValid(c, p) && (Seq.First(p) == next_np) && (Seq.Last(p) in nps_b);
+      var p_contradict := [np] + p;
+      reveal PathValid();
+      assert PathValid(c, p_contradict);
+      assert PathToNPSet(c, p_contradict, np, nps_b);
+      assert PathExistsToNPSet(c, np, nps_b);
+      assert false;
+    }
+  }
+
+  predicate PathBetweenNPSets(c: Circuit, p: seq<NP>, nps_a: set<NP>, nps_b: set<NP>)
+    requires c.Valid()
+  {
+    (|p| > 0) && PathValid(c, p) && (Seq.First(p) in nps_a) && (Seq.Last(p) in nps_b)
+  }
+
+  opaque ghost predicate PathExistsBetweenNPSets(c: Circuit, nps_a: set<NP>, nps_b: set<NP>)
+    requires c.Valid()
+  {
+    exists p: seq<NP> :: PathBetweenNPSets(c, p, nps_a, nps_b)
+  }
+
+  lemma NoPathExistsBetweenNPSetsToNoPathExists(c: Circuit, nps_a: set<NP>, nps_b: set<NP>, np_a: NP, np_b: NP)
+    requires c.Valid()
+    requires np_a in nps_a
+    requires np_b in nps_b
+    requires !PathExistsBetweenNPSets(c, nps_a, nps_b)
+    ensures !PathExists(c, np_a, np_b)
+  {
+    reveal PathExistsBetweenNPSets();
+    reveal PathExists();
+    if PathExists(c, np_a, np_b) {
+      var p := PathExistsToPath(c, np_a, np_b);
+      assert PathBetweenNPSets(c, p, nps_a, nps_b);
+    }
+  }
+
+  lemma NoPathExistsBetweenNPSetsToToNPSet(c: Circuit, nps_a: set<NP>, nps_b: set<NP>, np: NP)
+    requires c.Valid()
+    requires !PathExistsBetweenNPSets(c, nps_a, nps_b)
+    requires np in nps_a
+    ensures !PathExistsToNPSet(c, np, nps_b)
+  {
+    reveal PathExistsBetweenNPSets();
+    reveal PathExistsToNPSet();
+  }
+
+  predicate PathFromTo(c: Circuit, p: seq<NP>, a: NP, b: NP)
+    requires c.Valid()
+  {
+    PathValid(c, p) && |p| > 0 && Seq.First(p) == a && Seq.Last(p) == b && PathValid(c, p)
+  }
+
+  function JoinPaths(c: Circuit, pa: seq<NP>, pb: seq<NP>): (p: seq<NP>)
+    requires c.Valid()
+    requires PathNonZeroValid(c, pa)
+    requires PathNonZeroValid(c, pb)
+    requires Seq.Last(pa) == Seq.First(pb)
+    ensures PathValid(c, p)
+  {
+    reveal PathValid();
+    pa + pb[1..]
+  }
+
+  lemma PathsNoIntersection(c: Circuit, nps_a: set<NP>, nps_b: set<NP>, p_a: seq<NP>, p_b: seq<NP>)
+    requires c.Valid()
+    requires PathNonZeroValid(c, p_a)
+    requires PathNonZeroValid(c, p_b)
+    requires !PathExistsBetweenNPSets(c, nps_a, nps_b)
+    requires Seq.Last(p_a) in nps_b
+    requires Seq.First(p_b) in nps_a
+    ensures Seq.ToSet(p_a) !! Seq.ToSet(p_b)
+  {
+    if exists np :: np in p_a && np in p_b {
+      var np :| np in p_a && np in p_b;
+      var index_a := Seq.IndexOf(p_a, np);
+      var index_b := Seq.IndexOf(p_b, np);
+      var p_c := ValidPathSegment(c, p_a, index_a, |p_a|);
+      var p_d := ValidPathSegment(c, p_b, 0, index_b+1);
+      var p_joined := JoinPaths(c, p_d, p_c);
+      assert PathFromTo(c, p_joined, Seq.First(p_b), Seq.Last(p_a));
+      reveal PathExistsBetweenNPSets();
+      assert PathExistsBetweenNPSets(c, nps_a, nps_b);
+      assert false;
+    }
+    reveal Seq.ToSet();
+  }
+
+  ghost opaque predicate PathCaught(c: Circuit, p: seq<NP>, catcher: set<NP>)
+    requires c.Valid()
+    requires PathNonZeroValid(c, p)
+    requires Seq.HasNoDuplicates(p)
+    decreases
+      |NodesNotInPath(c, p)|
+  {
+    var np := Seq.Last(p);
+    assert NPValid(c, np) by {
+      reveal PathValid();
+    }
+    if np in catcher then
+      true
+    else if c.NodeKind[np.n].CConst? then
+      true
+    else
+      reveal PathValid();
+      forall next_np: NP :: NPValid(c, next_np) && NPsConnected(c, Seq.Last(p), next_np) ==>
+        && var new_p := p + [next_np];
+        && (next_np !in p)
+        && assert PathValid(c, new_p) && |NodesNotInPath(c, new_p)| < |NodesNotInPath(c, p)| by {
+          AppendPathValid(c, p, next_np);
+          NodesNotInPathDecreases(c, p, next_np);
+        }
+        && assert Seq.HasNoDuplicates(new_p) by {
+          reveal Seq.HasNoDuplicates();
+        }
+        && PathCaught(c, new_p, catcher)
+  }
+
+  // Prove that if something Evaluates as EvalOK then the FI inputs catch the paths
+  // from the output.  These are two different ways of saying we're not missing any inputs
+  // and we don't have any loops.
+  // This proof connects them.
+
+  lemma EvaluateOkToPathCaught(c: Circuit, np: NP, fi: FI)
+    requires c.Valid()
+    requires NPValid(c, np)
+    requires FICircuitValid(c, fi)
+    requires Evaluate(c, np, fi).EvalOk?
+    ensures
+      var ending_set := fi.inputs.Keys + StateONPsFromSet(fi.state.Keys);
+      var p := [np];
+      && PathValid(c, p)
+      && Seq.HasNoDuplicates(p)
+      && PathCaught(c, p, ending_set)
+  {
+    if ONPValid(c, np) {
+      EvaluateONPOkToPathCaught(c, np, fi);
+    } else {
+      EvaluateINPOkToPathCaught(c, np, fi);
+    }
+  }
+
+  lemma EvaluateONPOkToPathCaught(c: Circuit, np: NP, fi: FI)
+    requires c.Valid()
+    requires FICircuitValid(c, fi)
+    requires ONPValid(c, np)
+    requires EvaluateONP(c, np, fi).EvalOk?
+    ensures
+      var ending_set := fi.inputs.Keys + StateONPsFromSet(fi.state.Keys);
+      var p := [np];
+      && PathValid(c, p)
+      && Seq.HasNoDuplicates(p)
+      && PathCaught(c, p, ending_set)
+  {
+    var path := [np];
+    LengthOneNoDuplicates(path);
+    reveal PathValid();
+    var p := [np];
+    assert PathValid(c, p);
+    EvaluateONPInnerOkToPathCaught(c, p, fi);
+  }
+
+  lemma EvaluateINPOkToPathCaught(c: Circuit, np: NP, fi: FI)
+    requires c.Valid()
+    requires FICircuitValid(c, fi)
+    requires INPValid(c, np)
+    requires EvaluateINP(c, np, fi).EvalOk?
+    ensures
+      var ending_set := fi.inputs.Keys + StateONPsFromSet(fi.state.Keys);
+      var p := [np];
+      && PathValid(c, p)
+      && Seq.HasNoDuplicates(p)
+      && PathCaught(c, p, ending_set)
+  {
+    var path := [np];
+    LengthOneNoDuplicates(path);
+    reveal PathValid();
+    EvaluateINPInnerOkToPathCaught(c, path, fi);
+  }
+
+  lemma EvaluateONPInnerOkToPathCaught(c: Circuit, p: seq<NP>, fi: FI)
+    requires c.Valid()
+    requires PathValid(c, p)
+    requires EvaluateONPInnerRequirements(c, p, fi)
+    requires EvaluateONPInner(c, p, fi).EvalOk?
+    decreases |NodesNotInPath(c, p)|, 4
+    ensures
+      var ending_set := fi.inputs.Keys + StateONPsFromSet(fi.state.Keys);
+      && PathCaught(c, p, ending_set)
+  {
+    var ending_set := fi.inputs.Keys + StateONPsFromSet(fi.state.Keys);
+    var head := Seq.Last(p);
+    var nk := c.NodeKind[head.n];
+    if head.n in fi.state {
+      assert nk.CSeq? by {
+        reveal FICircuitValid();
+      }
+      match nk
+        case CSeq() => {
+          reveal PathCaught();
+        }
+    } else {
+      match nk
+        case CXor() => EvaluateONPBinaryOkToPathCaught(c, p, fi);
+        case CAnd() => EvaluateONPBinaryOkToPathCaught(c, p, fi);
+        case CInv() => EvaluateONPUnaryOkToPathCaught(c, p, fi);
+        case CIden() => EvaluateONPUnaryOkToPathCaught(c, p, fi);
+        case CConst(b) => {
+          reveal PathCaught();
+        }
+        case CSeq() => {
+        }
+    }
+  }
+
+  lemma EvaluateONPBinaryOkToPathCaught(c: Circuit, path: seq<NP>, fi: FI)
+    requires EvaluateONPBinaryRequirements(c, path, fi)
+    requires EvaluateONPBinary(c, path, fi).EvalOk?
+    ensures
+      var ending_set := fi.inputs.Keys + StateONPsFromSet(fi.state.Keys);
+      && PathCaught(c, path, ending_set)
+    decreases |NodesNotInPath(c, path)|, 3
+  {
+    var ending_set := fi.inputs.Keys + StateONPsFromSet(fi.state.Keys);
+    var nk := c.NodeKind[path[|path|-1].n];
+    var head := Seq.Last(path);
+    assert NodeValid(c, head.n);
+    var inp_0 := NP(head.n, INPUT_0);
+    var inp_1 := NP(head.n, INPUT_1);
+    if inp_0 in path {
+    } else if inp_1 in path {
+    } else {
+      NodesNotInPathDecreases(c, path, inp_0);
+      NodesNotInPathDecreases(c, path, inp_1);
+      var new_path_0 := path + [inp_0];
+      var new_path_1 := path + [inp_1];
+      assert PathValid(c, new_path_0);
+      assert PathValid(c, new_path_1);
+      assert |NodesNotInPath(c, path + [inp_0])| < |NodesNotInPath(c, path)|;
+      StillHasNoDuplicates(path, inp_0);
+      StillHasNoDuplicates(path, inp_1);
+      EvaluateINPInnerOkToPathCaught(c, path + [inp_0], fi);
+      EvaluateINPInnerOkToPathCaught(c, path + [inp_1], fi);
+      assert PathCaught(c, path, ending_set) by {
+        reveal PathCaught();
+      }
+    }
+  }
+
+  lemma EvaluateONPUnaryOkToPathCaught(c: Circuit, path: seq<NP>, fi: FI)
+    requires EvaluateONPUnaryRequirements(c, path, fi)
+    requires EvaluateONPUnary(c, path, fi).EvalOk?
+    ensures
+      var ending_set := fi.inputs.Keys + StateONPsFromSet(fi.state.Keys);
+      && PathCaught(c, path, ending_set)
+    decreases |NodesNotInPath(c, path)|, 3
+  {
+    var ending_set := fi.inputs.Keys + StateONPsFromSet(fi.state.Keys);
+    var nk := c.NodeKind[path[|path|-1].n];
+    var head := Seq.Last(path);
+    assert NodeValid(c, head.n);
+    var inp_0 := NP(head.n, INPUT_0);
+    if inp_0 in path {
+    } else {
+      NodesNotInPathDecreases(c, path, inp_0);
+      var new_path_0 := path + [inp_0];
+      assert PathValid(c, new_path_0);
+      assert |NodesNotInPath(c, path + [inp_0])| < |NodesNotInPath(c, path)|;
+      StillHasNoDuplicates(path, inp_0);
+      EvaluateINPInnerOkToPathCaught(c, path + [inp_0], fi);
+      assert PathCaught(c, path, ending_set) by {
+        reveal PathCaught();
+      }
+    }
+  }
+
+  lemma EvaluateINPInnerOkToPathCaught(c: Circuit, path: seq<NP>, fi: FI)
+    requires EvaluateINPInnerRequirements(c, path, fi)
+    requires EvaluateINPInner(c, path, fi).EvalOk?
+    ensures
+      var ending_set := fi.inputs.Keys + StateONPsFromSet(fi.state.Keys);
+      && PathCaught(c, path, ending_set)
+    decreases |NodesNotInPath(c, path)|, 2
+  {
+    var head := path[|path|-1];
+    var tail := path[..|path|-1];
+    if head in fi.inputs {
+      reveal PathCaught();
+    } else {
+      if head in c.PortSource {
+        var onp := c.PortSource[head];
+        if onp in path {
+        } else {
+          reveal Circuit.Valid();
+          NodesNotInPathDecreases(c, path, onp);
+          StillHasNoDuplicates(path, onp);
+          AppendPathValid(c, path, onp);
+          EvaluateONPInnerOkToPathCaught(c, path + [onp], fi);
+          reveal PathCaught();
+        }
+      } else {
+      }
+    }
+  }
+
+  // Prove that prepending to the beginning of the path is fine, as long as their is no way of
+  // creating a loop.
+
+  lemma EvaluateONPInnerPrepend(c: Circuit, prefix: seq<NP>, p: seq<NP>, fi: FI)
+    requires EvaluateONPInnerRequirements(c, p, fi)
+    requires EvaluateONPInnerRequirements(c, prefix + p, fi)
+    requires
+      var new_p := prefix + p;
+      |prefix| > 0 ==> !PathExists(c, Seq.Last(new_p), Seq.Last(prefix))
+    ensures
+      EvaluateONPInner(c, p, fi) == EvaluateONPInner(c, prefix + p, fi)
+    decreases |NodesNotInPath(c, p)|, 4
+  {
+    var ending_set := fi.inputs.Keys + StateONPsFromSet(fi.state.Keys);
+    var head := Seq.Last(p);
+    var nk := c.NodeKind[head.n];
+    if head.n in fi.state {
+      assert nk.CSeq? by {
+        reveal FICircuitValid();
+      }
+      match nk
+        case CSeq() => {
+          reveal PathCaught();
+        }
+    } else {
+      match nk
+        case CXor() => EvaluateONPBinaryPrepend(c, prefix, p, fi);
+        case CAnd() => EvaluateONPBinaryPrepend(c, prefix, p, fi);
+        case CInv() => EvaluateONPUnaryPrepend(c, prefix, p, fi);
+        case CIden() => EvaluateONPUnaryPrepend(c, prefix, p, fi);
+        case CConst(b) => {
+          reveal PathCaught();
+        }
+        case CSeq() => {
+        }
+    }
+  }
+
+  lemma NextNodeInPathAndNewPathSame(c: Circuit, prefix: seq<NP>, path: seq<NP>, np: NP)
+    requires c.Valid()
+    requires PathNonZeroValid(c, path)
+    requires PathValid(c, prefix + path)
+    requires NPValid(c, np)
+    requires
+      reveal PathValid();
+      NPsConnected(c, Seq.Last(path), np)
+    requires
+      |prefix| > 0 ==> !PathExists(c, Seq.Last(path), Seq.Last(prefix))
+    ensures
+      var new_path := prefix + path;
+      && ((np in path) == (np in new_path))
+  {
+    var new_path := prefix + path;
+    reveal PathValid();
+    if |prefix| > 0 {
+      assert prefix == ValidPathSegment(c, new_path, 0, |prefix|);
+    }
+    assert PathValid(c, prefix);
+    assert np in path ==> np in new_path;
+    assert np !in path ==> np !in new_path by {
+      if np !in path && np in new_path {
+        var index: nat :| index < |prefix| && prefix[index] == np;
+        var p_contradict := [Seq.Last(path)] + prefix[index..];
+        assert PathValid(c, p_contradict);
+        reveal PathExists();
+        assert PathExists(c, Seq.Last(new_path), Seq.Last(prefix));
+        assert false;
+      }
+    }
+  }
+
+  lemma StillNoPathExists(c: Circuit, a: NP, b: NP, dest: NP)
+    requires c.Valid()
+    requires !PathExists(c, a, dest)
+    requires NPValid(c, a)
+    requires NPValid(c, b)
+    requires NPsConnected(c, a, b)
+    ensures
+      !PathExists(c, b, dest)
+  {
+    if PathExists(c, b, dest) {
+      var path := PathExistsToPath(c, b, dest);
+      var path_contradict := [a] + path;
+      reveal PathValid();
+      assert PathFromTo(c, path_contradict, a, dest);
+      reveal PathExists();
+      assert PathExists(c, a, dest);
+      assert false;
+    }
+  }
+
+  lemma LoopIsSame(c: Circuit, prefix: seq<NP>, path: seq<NP>, np: NP)
+    requires c.Valid()
+    requires np in path
+    requires Seq.HasNoDuplicates(prefix + path)
+    ensures
+      assert Seq.HasNoDuplicates(path) by {
+        SubSeqsNoDuplicates(prefix, path);
+      }
+      GetLoop(prefix + path, np) == GetLoop(path, np)
+  {
+    HasNoDuplicatesNotInBoth(prefix, path, np);
+    var long_path := prefix + path;
+    var long_index := Seq.IndexOf(long_path, np);
+    var index := Seq.IndexOf(path, np);
+    assert long_path[index + |prefix|] == np;
+    assert long_index == index + |prefix|;
+  }
+
+  lemma EvaluateONPBinaryPrepend(c: Circuit, prefix: seq<NP>, path: seq<NP>, fi: FI)
+    requires EvaluateONPBinaryRequirements(c, path, fi)
+    requires EvaluateONPBinaryRequirements(c, prefix + path, fi)
+    requires
+      var new_p := prefix + path;
+      |prefix| > 0 ==> !PathExists(c, Seq.Last(new_p), Seq.Last(prefix))
+    ensures
+      EvaluateONPBinary(c, path, fi) == EvaluateONPBinary(c, prefix + path, fi)
+    decreases |NodesNotInPath(c, path)|, 3
+  {
+    var ending_set := fi.inputs.Keys + StateONPsFromSet(fi.state.Keys);
+    var nk := c.NodeKind[path[|path|-1].n];
+    var head := Seq.Last(path);
+    assert NodeValid(c, head.n);
+    var inp_0 := NP(head.n, INPUT_0);
+    var inp_1 := NP(head.n, INPUT_1);
+    var new_path := prefix + path;
+    NextNodeInPathAndNewPathSame(c, prefix, path, inp_0);
+    NextNodeInPathAndNewPathSame(c, prefix, path, inp_1);
+    if inp_0 in path {
+      LoopIsSame(c, prefix, path, inp_0);
+      assert EvaluateONPBinary(c, path, fi) == EvaluateONPBinary(c, prefix + path, fi);
+    } else if inp_1 in path {
+      LoopIsSame(c, prefix, path, inp_1);
+      assert EvaluateONPBinary(c, path, fi) == EvaluateONPBinary(c, prefix + path, fi);
+    } else {
+      NodesNotInPathDecreases(c, path, inp_0);
+      NodesNotInPathDecreases(c, path, inp_1);
+      var new_path_0 := path + [inp_0];
+      var new_path_1 := path + [inp_1];
+      assert PathValid(c, new_path_0);
+      assert PathValid(c, new_path_1);
+      assert (prefix + path) + [inp_0] == prefix + (path + [inp_0]);
+      assert (prefix + path) + [inp_1] == prefix + (path + [inp_1]);
+      assert PathValid(c, prefix + new_path_0) by {reveal PathValid();}
+      assert PathValid(c, prefix + new_path_1) by {reveal PathValid();}
+      assert |NodesNotInPath(c, path + [inp_0])| < |NodesNotInPath(c, path)|;
+      StillHasNoDuplicates(path, inp_0);
+      StillHasNoDuplicates(path, inp_1);
+      StillHasNoDuplicates(prefix + path, inp_0);
+      StillHasNoDuplicates(prefix + path, inp_1);
+      if |prefix| > 0 {
+        StillNoPathExists(c, head, inp_0, Seq.Last(prefix));
+        StillNoPathExists(c, head, inp_1, Seq.Last(prefix));
+      }
+      EvaluateINPInnerPrepend(c, prefix, path + [inp_0], fi);
+      EvaluateINPInnerPrepend(c, prefix, path + [inp_1], fi);
+      assert EvaluateONPBinary(c, path, fi) == EvaluateONPBinary(c, prefix + path, fi);
+    }
+  }
+
+  lemma EvaluateONPUnaryPrepend(c: Circuit, prefix: seq<NP>, path: seq<NP>, fi: FI)
+    requires EvaluateONPUnaryRequirements(c, path, fi)
+    requires EvaluateONPUnaryRequirements(c, prefix + path, fi)
+    requires
+      var new_p := prefix + path;
+      |prefix| > 0 ==> !PathExists(c, Seq.Last(new_p), Seq.Last(prefix))
+    ensures
+      EvaluateONPUnary(c, path, fi) == EvaluateONPUnary(c, prefix + path, fi)
+    decreases |NodesNotInPath(c, path)|, 3
+  {
+    var ending_set := fi.inputs.Keys + StateONPsFromSet(fi.state.Keys);
+    var nk := c.NodeKind[path[|path|-1].n];
+    var head := Seq.Last(path);
+    assert NodeValid(c, head.n);
+    var inp_0 := NP(head.n, INPUT_0);
+    NextNodeInPathAndNewPathSame(c, prefix, path, inp_0);
+    if inp_0 in path {
+      LoopIsSame(c, prefix, path, inp_0);
+      assert EvaluateONPUnary(c, path, fi) == EvaluateONPUnary(c, prefix + path, fi);
+    } else {
+      NodesNotInPathDecreases(c, path, inp_0);
+      var new_path_0 := path + [inp_0];
+      assert (prefix + path) + [inp_0] == prefix + (path + [inp_0]);
+      assert PathValid(c, new_path_0);
+      assert PathValid(c, prefix + new_path_0) by {reveal PathValid();}
+      assert |NodesNotInPath(c, path + [inp_0])| < |NodesNotInPath(c, path)|;
+      StillHasNoDuplicates(path, inp_0);
+      StillHasNoDuplicates(prefix + path, inp_0);
+      if |prefix| > 0 {
+        StillNoPathExists(c, head, inp_0, Seq.Last(prefix));
+      }
+      EvaluateINPInnerPrepend(c, prefix, path + [inp_0], fi);
+    }
+  }
+
+  lemma EvaluateINPInnerPrepend(c: Circuit, prefix: seq<NP>, path: seq<NP>, fi: FI)
+    requires EvaluateINPInnerRequirements(c, path, fi)
+    requires EvaluateINPInnerRequirements(c, prefix + path, fi)
+    requires
+      var new_p := prefix + path;
+      |prefix| > 0 ==> !PathExists(c, Seq.Last(new_p), Seq.Last(prefix))
+    ensures
+      EvaluateINPInner(c, path, fi) == EvaluateINPInner(c, prefix + path, fi)
+    decreases |NodesNotInPath(c, path)|, 2
+  {
+    var head := path[|path|-1];
+    var tail := path[..|path|-1];
+    if head in fi.inputs {
+    } else {
+      if head in c.PortSource {
+        var onp := c.PortSource[head];
+        assert ONPValid(c, onp) by {
+          reveal Circuit.Valid();
+        }
+        NextNodeInPathAndNewPathSame(c, prefix, path, onp);
+        if onp in path {
+          LoopIsSame(c, prefix, path, onp);
+        } else {
+          reveal Circuit.Valid();
+          NodesNotInPathDecreases(c, path, onp);
+          StillHasNoDuplicates(path, onp);
+          StillHasNoDuplicates(prefix + path, onp);
+          AppendPathValid(c, path, onp);
+          AppendPathValid(c, prefix + path, onp);
+          assert (prefix + path) + [onp] == prefix + (path + [onp]);
+          if |prefix| > 0 {
+            StillNoPathExists(c, head, onp, Seq.Last(prefix));
+          }
+          EvaluateONPInnerPrepend(c, prefix, path + [onp], fi);
+          reveal PathCaught();
+        }
+      } else {
+      }
+    }
+  }
+
+
+}
