Path2.dfy
@@ -1,0 +1,210 @@
+module Path2 {
+
+  import opened Circ
+  import opened Eval
+  import opened MapFunction
+  import opened Utils
+  import opened Path
+
+  // Prove that if there are no paths from onp to inps then we can remove inps from fi with
+  // no effect on the outcome.
+
+  lemma EvaluateReduceFI(c: Circuit, np: NP, fi: FI, removed: set<NP>)
+    requires c.Valid()
+    requires NPValid(c, np)
+    requires FICircuitValid(c, fi)
+    requires !PathExistsToNPSet(c, np, removed)
+    ensures
+      var reduced_fi := FI(fi.inputs - removed, fi.state);
+      reveal FICircuitValid();
+      Evaluate(c, np, fi) == Evaluate(c, np, reduced_fi)
+  {
+    var reduced_fi := FI(fi.inputs - removed, fi.state);
+    reveal FICircuitValid();
+    if ONPValid(c, np) {
+      EvaluateONPReduceFI(c, np, fi, removed);
+    } else {
+      EvaluateINPReduceFI(c, np, fi, removed);
+    }
+  }
+
+  lemma EvaluateONPReduceFI(c: Circuit, np: NP, fi: FI, removed: set<NP>)
+    requires c.Valid()
+    requires FICircuitValid(c, fi)
+    requires ONPValid(c, np)
+    requires !PathExistsToNPSet(c, np, removed)
+    ensures
+      var reduced_fi := FI(fi.inputs - removed, fi.state);
+      reveal FICircuitValid();
+      EvaluateONP(c, np, fi) == EvaluateONP(c, np, reduced_fi)
+  {
+    reveal FICircuitValid();
+    var path := [np];
+    LengthOneNoDuplicates(path);
+    reveal PathValid();
+    var p := [np];
+    assert PathValid(c, p);
+    EvaluateONPInnerReduceFI(c, p, fi, removed);
+  }
+
+  lemma EvaluateINPReduceFI(c: Circuit, np: NP, fi: FI, removed: set<NP>)
+    requires c.Valid()
+    requires FICircuitValid(c, fi)
+    requires INPValid(c, np)
+    requires !PathExistsToNPSet(c, np, removed)
+    ensures
+      var reduced_fi := FI(fi.inputs - removed, fi.state);
+      reveal FICircuitValid();
+      EvaluateINP(c, np, fi) == EvaluateINP(c, np, reduced_fi)
+  {
+    reveal FICircuitValid();
+    var path := [np];
+    LengthOneNoDuplicates(path);
+    reveal PathValid();
+    EvaluateINPInnerReduceFI(c, path, fi, removed);
+  }
+
+  lemma EvaluateONPInnerReduceFI(c: Circuit, p: seq<NP>, fi: FI, removed: set<NP>)
+    requires c.Valid()
+    requires PathValid(c, p)
+    requires EvaluateONPInnerRequirements(c, p, fi)
+    requires !PathExistsToNPSet(c, Seq.Last(p), removed)
+    ensures
+      var reduced_fi := FI(fi.inputs - removed, fi.state);
+      reveal FICircuitValid();
+      EvaluateONPInner(c, p, fi) == EvaluateONPInner(c, p, reduced_fi)
+    decreases |NodesNotInPath(c, p)|, 4
+  {
+    var reduced_fi := FI(fi.inputs - removed, fi.state);
+    reveal FICircuitValid();
+    var head := Seq.Last(p);
+    var nk := c.NodeKind[head.n];
+    if head.n in fi.state {
+      assert head.n in reduced_fi.state;
+      assert nk.CSeq? by {
+        reveal FICircuitValid();
+      }
+      match nk
+        case CSeq() => {
+          reveal PathCaught();
+        }
+    } else {
+      match nk
+        case CXor() => EvaluateONPBinaryReduceFI(c, p, fi, removed);
+        case CAnd() => EvaluateONPBinaryReduceFI(c, p, fi, removed);
+        case CInv() => EvaluateONPUnaryReduceFI(c, p, fi, removed);
+        case CIden() => EvaluateONPUnaryReduceFI(c, p, fi, removed);
+        case CConst(b) => {
+          reveal PathCaught();
+        }
+        case CSeq() => {
+        }
+    }
+  }
+
+  lemma EvaluateONPBinaryReduceFI(c: Circuit, path: seq<NP>, fi: FI, removed: set<NP>)
+    requires EvaluateONPBinaryRequirements(c, path, fi)
+    requires !PathExistsToNPSet(c, Seq.Last(path), removed)
+    ensures
+      var reduced_fi := FI(fi.inputs - removed, fi.state);
+      reveal FICircuitValid();
+      EvaluateONPBinary(c, path, fi) == EvaluateONPBinary(c, path, reduced_fi)
+    decreases |NodesNotInPath(c, path)|, 3
+  {
+    var reduced_fi := FI(fi.inputs - removed, fi.state);
+    reveal FICircuitValid();
+    var nk := c.NodeKind[path[|path|-1].n];
+    var head := Seq.Last(path);
+    assert NodeValid(c, head.n);
+    var inp_0 := NP(head.n, INPUT_0);
+    var inp_1 := NP(head.n, INPUT_1);
+    if inp_0 in path {
+    } else if inp_1 in path {
+    } else {
+      NodesNotInPathDecreases(c, path, inp_0);
+      NodesNotInPathDecreases(c, path, inp_1);
+      var new_path_0 := path + [inp_0];
+      var new_path_1 := path + [inp_1];
+      assert PathValid(c, new_path_0);
+      assert PathValid(c, new_path_1);
+      assert |NodesNotInPath(c, path + [inp_0])| < |NodesNotInPath(c, path)|;
+      StillHasNoDuplicates(path, inp_0);
+      StillHasNoDuplicates(path, inp_1);
+      StillNoPathExistsToNPSet(c, Seq.Last(path), inp_0, removed);
+      StillNoPathExistsToNPSet(c, Seq.Last(path), inp_1, removed);
+      EvaluateINPInnerReduceFI(c, path + [inp_0], fi, removed);
+      EvaluateINPInnerReduceFI(c, path + [inp_1], fi, removed);
+    }
+  }
+
+  lemma EvaluateONPUnaryReduceFI(c: Circuit, path: seq<NP>, fi: FI, removed: set<NP>)
+    requires EvaluateONPUnaryRequirements(c, path, fi)
+    requires !PathExistsToNPSet(c, Seq.Last(path), removed)
+    ensures
+      var reduced_fi := FI(fi.inputs - removed, fi.state);
+      reveal FICircuitValid();
+      EvaluateONPUnary(c, path, fi) == EvaluateONPUnary(c, path, reduced_fi)
+    decreases |NodesNotInPath(c, path)|, 3
+  {
+    var reduced_fi := FI(fi.inputs - removed, fi.state);
+    reveal FICircuitValid();
+    var ending_set := fi.inputs.Keys + StateONPsFromSet(fi.state.Keys);
+    var nk := c.NodeKind[path[|path|-1].n];
+    var head := Seq.Last(path);
+    assert NodeValid(c, head.n);
+    var inp_0 := NP(head.n, INPUT_0);
+    if inp_0 in path {
+    } else {
+      NodesNotInPathDecreases(c, path, inp_0);
+      var new_path_0 := path + [inp_0];
+      assert PathValid(c, new_path_0);
+      assert |NodesNotInPath(c, path + [inp_0])| < |NodesNotInPath(c, path)|;
+      StillHasNoDuplicates(path, inp_0);
+      StillNoPathExistsToNPSet(c, Seq.Last(path), inp_0, removed);
+      EvaluateINPInnerReduceFI(c, path + [inp_0], fi, removed);
+    }
+  }
+
+  lemma EvaluateINPInnerReduceFI(c: Circuit, path: seq<NP>, fi: FI, removed: set<NP>)
+    requires EvaluateINPInnerRequirements(c, path, fi)
+    requires !PathExistsToNPSet(c, Seq.Last(path), removed)
+    ensures
+      var reduced_fi := FI(fi.inputs - removed, fi.state);
+      reveal FICircuitValid();
+      EvaluateINPInner(c, path, fi) == EvaluateINPInner(c, path, reduced_fi)
+    decreases |NodesNotInPath(c, path)|, 2
+  {
+    var reduced_fi := FI(fi.inputs - removed, fi.state);
+    reveal FICircuitValid();
+    var head := path[|path|-1];
+    var tail := path[..|path|-1];
+    if head in fi.inputs {
+      assert head !in removed by {
+        if head in removed {
+          reveal PathExistsToNPSet();
+          var p_contradict := [head];
+          reveal PathValid();
+          assert PathToNPSet(c, p_contradict, head, removed);
+          assert false;
+        }
+      }
+      assert head in reduced_fi.inputs;
+    } else {
+      if head in c.PortSource {
+        var onp := c.PortSource[head];
+        if onp in path {
+        } else {
+          reveal Circuit.Valid();
+          NodesNotInPathDecreases(c, path, onp);
+          StillHasNoDuplicates(path, onp);
+          AppendPathValid(c, path, onp);
+          StillNoPathExistsToNPSet(c, Seq.Last(path), onp, removed);
+          EvaluateONPInnerReduceFI(c, path + [onp], fi, removed);
+          reveal PathCaught();
+        }
+      } else {
+      }
+    }
+  }
+
+}
