SelfConnectEval.dfy
@@ -1,4 +1,4 @@
-module ConnectEval {
+module SelfConnectEval {
 
   import opened Circ
   import opened Scuf
@@ -6,6 +6,8 @@ module ConnectEval {
   import opened MapFunction
   import opened Eval
   import opened Subcircuit
+  import opened ConservedSubcircuit
+  import opened SelfConnectEval2
 
   ghost predicate ConnectRequirements(c: Circuit, s: Scuf, conn: InternalConnection, fi: FI)
   {
@@ -21,140 +23,6 @@ module ConnectEval {
     //&& FICircuitValid(new_c, fi)
   }
 
-  //lemma EvaluateONPInnerFirstPass(c: Circuit, s: Scuf, conn: InternalConnection, fi: FI, path: seq<NP>)
-  //  requires
-  //    var (new_c, new_s) := ConnectCircuitScufImpl(c, s, conn);
-  //    && EvaluateONPInnerRequirements(new_c, path, fi)
-  //    && PathInSubcircuit(path, s.sc)
-  //  ensures
-  //    var (new_c, new_s) := ConnectCircuitScufImpl(c, s, conn);
-  //    var fi_first_pass := conn.FIFirstPass(s.mp, fi);
-  //    && var np := Seq.Last(path);
-  //    && (EvaluateONPInner(new_c, path, fi) == EvaluateONPInner(new_c, path, fi_first_pass))
-  //  decreases
-  //    var (new_c, new_s) := ConnectCircuitScufImpl(c, s, conn);
-  //    |NodesNotInPath(new_c, path)|, 6
-  //{
-  //}
-  lemma EvaluateSelfConnectOldONP(c: Circuit, s: Scuf, conn: InternalConnection, np: NP, fi: FI)
-    //
-    // Here we need to prove that when we take a circuit and connect some of the input points to
-    // other nodes it doesn't effect the evaluation.
-    // This is because at the input points the evaluation is terminated.
-    //
-    requires c.Valid()
-    requires s.Valid(c)
-    requires conn.Valid()
-    requires ScufConnectionConsistent(c, s, conn)
-    requires FIValid(fi, s.mp.inputs, s.mp.state)
-    requires NPValid(c, np)
-    requires np in s.mp.outputs || np in StateINPs(s.mp.state)
-    ensures
-      var (new_c, new_s) := ConnectCircuitScufImpl(c, s, conn);
-      && FICircuitValid(new_c, fi)
-      && (Evaluate(new_c, np, fi) == Evaluate(c, np, fi))
-
-  lemma EvaluateSelfConnectFirstPassONP(c: Circuit, s: Scuf, conn: InternalConnection, np: NP, fi: FI)
-    //
-    // Here we prove that if when we evaluate one of the outputs that we have connected to an input,
-    // the result of the evaluation is not effected is we remove the connected inputs from the
-    // termination points.
-    // This is true because we enforce that there are not paths from the connected outputs to the connected
-    // inputs.
-    //
-    requires ConnectRequirements(c, s, conn, fi)
-    requires
-      var (new_c, new_s) := ConnectCircuitScufImpl(c, s, conn);
-      && NPValid(new_c, np)
-      && (np in conn.GetConnectedOutputs(s.mp))
-    ensures
-      var (new_c, new_s) := ConnectCircuitScufImpl(c, s, conn);
-      var fi_first_pass := conn.FIFirstPass(s.mp, fi);
-      && FICircuitValid(new_c, fi)
-      && FICircuitValid(new_c, fi_first_pass)
-      && (Evaluate(new_c, np, fi_first_pass) == Evaluate(new_c, np, fi))
-
-  lemma EvaluateSelfConnectSecondPassONP(c: Circuit, s: Scuf, conn: InternalConnection, np: NP, fi: FI)
-    //
-    // Here we prove that if when we evaluate an output using inputs created by fi_second_pass
-    // it is equivalent to using the fi inputs.
-    //
-    // The different between these two inputs is that `fi` does not contain elements from the connected
-    // inputs so to prove this we need to show that the values in fi_second_pass match match the values
-    // that are calculated using fi.
-    //
-    requires ConnectRequirements(c, s, conn, fi)
-    requires
-      var (new_c, new_s) := ConnectCircuitScufImpl(c, s, conn);
-      && NPValid(new_c, np)
-      && (np in new_s.mp.outputs || np in StateINPs(new_s.mp.state))
-    ensures
-      var (new_c, new_s) := ConnectCircuitScufImpl(c, s, conn);
-      var fi_second_pass := conn.FISecondPass(s.mp, s.uf, fi);
-      && FICircuitValid(new_c, fi)
-      && FICircuitValid(new_c, fi_second_pass)
-      && (Evaluate(new_c, np, fi_second_pass) == Evaluate(new_c, np, fi))
-
-  //lemma EvaluateSelfConnectFirstPass(c: Circuit, s: Scuf, conn: InternalConnection, np: NP, fi: FI)
-  //  //
-  //  // Here we prove that our evaluation of the circuit matches the UF model.
-  //  // We know that the old scuf is still valid but we still need to prove that the updated
-  //  // update function matches this conserved behavior.
-  //  //
-  //  requires ConnectRequirements(c, s, conn, fi)
-  //  requires
-  //    var (new_c, new_s) := ConnectCircuitScufImpl(c, s, conn);
-  //    && NPValid(new_c, np)
-  //    && (np in conn.GetConnectedOutputs(s.mp))
-  //    && s.SomewhatValidRelaxInputs(new_c)
-  //    && new_s.SomewhatValidRelaxInputs(new_c)
-  //  ensures
-  //    var (new_c, new_s) := ConnectCircuitScufImpl(c, s, conn);
-  //    var fi_first_pass := conn.FIFirstPass(s.mp, fi);
-  //    && FICircuitValid(new_c, fi)
-  //    && FICircuitValid(new_c, fi_first_pass)
-  //    && assert np in new_s.mp.outputs by {
-  //      reveal Seq.ToSet();
-  //    }
-  //    && (Evaluate(new_c, np, fi) == EvalOk(MFLookup(new_s, fi, np)))
-  //{
-  //  var (new_c, new_s) := ConnectCircuitScufImpl(c, s, conn);
-  //  var fi_first_pass := conn.FIFirstPass(s.mp, fi);
-
-  //  assert FICircuitValid(new_c, fi ) by {
-  //    assert FIValid(fi, new_s.mp.inputs, new_s.mp.state);
-  //    ScufValidFiValidToFICircuitValid(new_c, new_s, fi);
-  //    reveal FICircuitValid();
-  //  }
-
-  //  assert FICircuitValid(new_c, fi_first_pass) by {
-  //    assert FIValid(fi_first_pass, s.mp.inputs, s.mp.state);
-  //    ScufValidFiValidToFICircuitValid(new_c, s, fi_first_pass);
-  //    reveal FICircuitValid();
-  //  }
-
-  //  calc {
-  //    Evaluate(new_c, np, fi);
-  //    {
-  //      EvaluateSelfConnectFirstPassONP(c, s, conn, np, fi);
-  //    }
-  //    Evaluate(new_c, np, fi_first_pass);
-  //    {
-  //      EvaluateSelfConnectOldONP(c, s, conn, np, fi_first_pass);
-  //    }
-  //    Evaluate(c, np, fi_first_pass);
-  //    {
-  //      assert s.Valid(c);
-  //      reveal Seq.ToSet();
-  //      reveal Scuf.EvaluatesCorrectly();
-  //    }
-  //    EvalOk(MFLookup(s, fi_first_pass, np));
-  //    {
-  //      SelfConnectFirstPassMFLookup(s, conn, np, fi);
-  //    }
-  //    EvalOk(MFLookup(new_s, fi, np));
-  //  }
-  //}
 
   lemma EvaluateSelfConnect(c: Circuit, s: Scuf, conn: InternalConnection, np: NP, fi: FI)
     requires ConnectRequirements(c, s, conn, fi)
@@ -200,7 +68,7 @@ module ConnectEval {
     calc {
       Evaluate(new_c, np, fi);
       {
-        EvaluateSelfConnectSecondPassONP(c, s, conn, np, fi);
+        EvaluateWithActual(c, s, conn, np, fi);
       }
       Evaluate(new_c, np, fi_second_pass);
       {
