SelfConnectEval2.dfy
@@ -1,0 +1,706 @@
+module SelfConnectEval2 {
+
+  import opened Circ
+  import opened Scuf
+  import opened SelfConnect
+  import opened MapFunction
+  import opened Eval
+  import opened Utils
+  import opened Subcircuit
+  import opened ConservedSubcircuit
+  import opened Path
+  import opened Path2
+
+  // At the toplevel we're trying to prove that when we connect some outputs to some inputs we the resulting
+  // circuit is consistent with the updated UpdateFunction.
+
+
+  // The new update function does:
+  // 1) Set all the recycled inputs to 0.
+  // 2) Run the old update function to get the outputs. The output values from this are correct for the connected outputs
+  //    because there are no connections from the inputs to the outputs internally.
+  // 3) Set the recycles inputs to the proper values from the outputs.
+  // 4) Run the old update function again.
+
+
+  // Proof steps.
+  // 1) Prove that Evaluation using fi_actual matches Evaluation using fi.
+  //    Evaluate(new_c, np, fi) == Evaluate(new_c, np, fi_with_real_outputs)
+  // 2) Prove that the result for c and new_c will be the same if all the connections are in fi
+  //    Evaluate(new_c, np, fi_with_real_outputs) == Evaluate(c, np, fi_with_real_outputs)
+  // 2) Prove that Evaluation using fi_actual matches old_update(fi_actual)
+  //    Evaluate(c, np, fi_with_real_outputs) == EvalOk(UFOld(fi_with_real_outputs))
+  // 3) Prove that old_update(fi_actual) == new_update(fi)
+  //    EvalOk(UFOld(fi_with_real_outputs)) == EvalOk(UFNew(fi))
+  //
+  // Thus we get Evaluate(new_c, np, fi) == EvalOk(UFNew(fi))
+
+  // (1) is probably going to be the hardest.
+  // Having a different FI is only going to have an effect when we're at an INP that is in fi_with_real_inputs
+  // but not in fi.
+  // At this point we know that EvaluateINP(new, path, fi_with_real_outputs) is just EvalOk(fi_with_real_outputs[inp])
+  // however we need to prove this is the same with fi.
+  // It will be EvaluateONP(new, path + corresponding_onp, fi).  We need to be able to prove that if onp is in the connected outputs
+  // that
+  // a) EvaluateONP(new_c, path, fi) == EvaluateONP(new_c, path, fi_with_fake_outputs)
+  // b) EvaluateONP(new_c, path, fi_with_fake_outputs) == EvaluateONP(c, path, fi_with_fake_outputs)
+  // c) EvaluateONP(c, path, fi_with_fake_outputs) == EvalOk(UFOld(fi_with_fake_outputs))
+  // d) EvalOK(UFOld(fi_with_real_outputs)) == EvalOK(UFOld(fi_with_fake_outputs))) if onp is in connected outputs.
+
+  lemma EvaluateSelfConnectOldONP(c: Circuit, s: Scuf, conn: InternalConnection, np: NP, fi: FI)
+    //
+    // Here we need to prove that when we take a circuit and connect some of the input points to
+    // other nodes it doesn't effect the evaluation.
+    // This is because at the input points the evaluation is terminated.
+    //
+    requires c.Valid()
+    requires s.Valid(c)
+    requires conn.Valid()
+    requires ScufConnectionConsistent(c, s, conn)
+    requires FIValid(fi, s.mp.inputs, s.mp.state)
+    requires NPValid(c, np)
+    requires np in s.mp.outputs || np in StateINPs(s.mp.state)
+    ensures
+      var (new_c, new_s) := ConnectCircuitScufImpl(c, s, conn);
+      && FICircuitValid(new_c, fi)
+      && FICircuitValid(c, fi)
+      && (Evaluate(new_c, np, fi) == Evaluate(c, np, fi))
+  {
+    var (new_c, new_s) := ConnectCircuitScufImpl(c, s, conn);
+    assert ConservedValid(c, new_c, s, fi) by {
+      assert c.Valid();
+      assert new_c.Valid();
+      assert s.Valid(c);
+      assert SubcircuitWeaklyConserved(c, new_c, s.sc);
+      assert (Seq.ToSet(s.mp.inputs) == fi.inputs.Keys);
+      assert (Seq.ToSet(s.mp.state) == fi.state.Keys);
+      assert OutputsInFOutputs(new_c, s) by {
+        reveal Scuf.SomewhatValidRelaxInputs();
+        assert OutputsInFOutputs(c, s);
+        reveal ConnOutputs();
+        assert NoNewExternalConnections(c, new_c, s.sc);
+        reveal NoNewExternalConnections();
+        assert ConnOutputs(c, s.sc) == ConnOutputs(new_c, s.sc);
+      }
+    }
+    assert np.n in s.sc by {
+      reveal NPsInSc();
+      FOutputsInSc(c, s);
+      reveal Seq.ToSet();
+      if np in s.mp.outputs {
+        assert np.n in s.sc;
+      }
+      if np in StateINPs(s.mp.state) {
+        assert np.n in s.sc;
+      }
+    }
+    EvaluateConserved(c, new_c, s, np, fi);
+  }
+
+  lemma EvaluateWithActual(c: Circuit, s: Scuf, conn: InternalConnection, np: NP, fi: FI)
+    requires c.Valid()
+    requires s.Valid(c)
+    requires conn.Valid()
+    requires ScufConnectionConsistent(c, s, conn)
+    requires
+      && var (new_c, new_s) := ConnectCircuitScufImpl(c, s, conn);
+      && FIValid(fi, new_s.mp.inputs, new_s.mp.state)
+      && var fi_second_pass := conn.FISecondPass(s.mp, s.uf, fi);
+      && (np in s.mp.outputs || np in StateINPs(s.mp.state))
+    ensures
+      var (new_c, new_s) := ConnectCircuitScufImpl(c, s, conn);
+      var fi_second_pass := conn.FISecondPass(s.mp, s.uf, fi);
+      && (Evaluate(new_c, np, fi_second_pass) == Evaluate(new_c, np, fi))
+  {
+    if ONPValid(c, np) {
+      EvaluateONPInnerSelfConnect(c, s, conn, [np], fi);
+    } else {
+      EvaluateINPInnerSelfConnect(c, s, conn, [np], fi);
+    }
+  }
+
+
+  lemma EvaluateONPInnerConnectedOutputs(c: Circuit, s: Scuf, conn: InternalConnection, path: seq<NP>, fi: FI, outputs: seq<bool>)
+    //
+    // Here we prove that if when we evaluate one of the outputs that we have connected to an input,
+    // the result of the evaluation is not effected is we remove the connected inputs from the
+    // termination points.
+    // This is true because we enforce that there are not paths from the connected outputs to the connected
+    // inputs.
+    //
+    requires c.Valid()
+    requires s.Valid(c)
+    requires conn.Valid()
+    requires ScufConnectionConsistent(c, s, conn)
+    requires
+      var (new_c, new_s) := ConnectCircuitScufImpl(c, s, conn);
+      && FIValid(fi, new_s.mp.inputs, new_s.mp.state)
+      && (|outputs| == |s.mp.outputs|)
+      && var fi_pass := conn.FIFromOutputs(s.mp, fi, outputs);
+      && EvaluateONPInnerRequirements(new_c, path, fi)
+      && EvaluateONPInnerRequirements(new_c, path, fi_pass)
+      && PathValid(new_c, path)
+      && NPValid(new_c, Seq.Last(path))
+      && (|path| > 1 ==> !PathExists(new_c, Seq.Last(path), path[|path|-2]))
+      && (Seq.Last(path) in conn.GetConnectedOutputs(s.mp))
+    ensures
+      var (new_c, new_s) := ConnectCircuitScufImpl(c, s, conn);
+      var fi_pass := conn.FIFromOutputs(s.mp, fi, outputs);
+      reveal FICircuitValid();
+      && (EvaluateONPInner(new_c, path, fi_pass) == EvaluateONPInner(new_c, path, fi))
+      && reveal Seq.ToSet();
+      && (EvaluateONPInner(new_c, path, fi_pass) == EvalOk(MFLookup(s, fi_pass, Seq.Last(path))))
+  {
+    var (new_c, new_s) := ConnectCircuitScufImpl(c, s, conn);
+    var np := Seq.Last(path);
+    var fi_pass := conn.FIFromOutputs(s.mp, fi, outputs);
+    var onps := conn.GetConnectedOutputs(s.mp);
+    var inps := conn.GetConnectedInputs(s.mp);
+    assert Seq.ToSet(new_s.mp.inputs) == Seq.ToSet(s.mp.inputs) - inps;
+    assert fi == FI(fi_pass.inputs - inps, fi_pass.state) by {
+      assert fi.state == fi_pass.state;
+      var output_width := |s.mp.outputs|;
+      //var fake_output := seq(output_width, (index: nat) requires index < output_width => false);
+      var sni := new_s.mp.fi2si(fi);
+      conn.NIO2I2NI(sni.inputs, outputs);
+      assert fi.inputs.Keys == fi_pass.inputs.Keys - inps;
+      assert fi.inputs == fi_pass.inputs -inps by {
+        forall np | np in fi.inputs
+          ensures fi.inputs[np] == fi_pass.inputs[np]
+        {
+          conn.FIFromOutputsMatchingKeyMatchingValue(s.mp, s.uf, fi, outputs);
+        }
+      }
+    }
+    assert ONPsValid(c, onps) && ONPsValid(new_c, onps) by {
+      ScufFOutputsAreValid(c, s);
+      reveal Seq.ToSet();
+      reveal ONPsValid();
+    }
+    assert !PathExistsBetweenNPSets(new_c, onps, inps) by {
+      reveal ScufConnectionConsistent();
+      assert ONPsValid(c, onps);
+      StillNoPathExistsBetweenNPSets(c, new_c, onps, inps);
+    }
+    assert FICircuitValid(new_c, fi_pass) by {
+      reveal FICircuitValid();
+    }
+    NoPathExistsBetweenNPSetsToToNPSet(new_c, onps, inps, Seq.Last(path));
+    EvaluateONPInnerReduceFI(new_c, path, fi_pass, inps);
+    assert fi == FI(fi_pass.inputs - inps, fi_pass.state);
+    assert EvaluateONPInner(new_c, path, fi) == EvaluateONPInner(new_c, path, fi_pass);
+    assert Seq.HasNoDuplicates([Seq.Last(path)]) && PathValid(new_c, [Seq.Last(path)]) by {
+      reveal Seq.HasNoDuplicates();
+      reveal PathValid();
+    }
+    calc {
+      EvaluateONPInner(new_c, path, fi_pass);
+      {
+        reveal Seq.HasNoDuplicates();
+        reveal PathValid();
+        var prefix := if |path| > 1 then ValidPathSegment(new_c, path, 0, |path|-1) else [];
+        EvaluateONPInnerPrepend(new_c, prefix, [Seq.Last(path)], fi_pass);
+        assert path == prefix + [Seq.Last(path)];
+      }
+      EvaluateONPInner(new_c, [Seq.Last(path)], fi_pass);
+      Evaluate(new_c, Seq.Last(path), fi_pass);
+      {
+        reveal InternalConnection.Valid();
+        EvaluateSelfConnectOldONP(c, s, conn, Seq.Last(path), fi_pass);
+      }
+      Evaluate(c, Seq.Last(path), fi_pass);
+      {
+        assert s.Valid(c);
+        reveal InternalConnection.Valid();
+        reveal Scuf.EvaluatesCorrectly();
+      }
+      EvalOk(MFLookup(s, fi_pass, Seq.Last(path)));
+    }
+  }
+
+  ghost predicate EvaluateINPInnerSelfConnectRequirements(c: Circuit, s: Scuf, conn: InternalConnection, path: seq<NP>, fi: FI)
+  {
+    && c.Valid()
+    && s.Valid(c)
+    && conn.Valid()
+    && ScufConnectionConsistent(c, s, conn)
+    && var (new_c, new_s) := ConnectCircuitScufImpl(c, s, conn);
+    && FIValid(fi, new_s.mp.inputs, new_s.mp.state)
+    && var fi_second_pass := conn.FISecondPass(s.mp, s.uf, fi);
+    && EvaluateINPInnerRequirements(new_c, path, fi_second_pass)
+    && EvaluateINPInnerRequirements(new_c, path, fi)
+  }
+
+  lemma EvaluateINPInnerSelfConnectHelperA(c: Circuit, s: Scuf, conn: InternalConnection, path: seq<NP>, fi: FI)
+    requires EvaluateINPInnerSelfConnectRequirements(c, s, conn, path, fi)
+    requires (Seq.Last(path) !in fi.inputs)
+    requires PathValid(c, path)
+    requires 
+      var fi_second_pass := conn.FISecondPass(s.mp, s.uf, fi);
+      && (Seq.Last(path) in fi_second_pass.inputs)
+    ensures
+      var (new_c, new_s) := ConnectCircuitScufImpl(c, s, conn);
+      var onp: NP := new_c.PortSource[Seq.Last(path)];
+      && PathValid(new_c, path + [onp])
+      && Seq.HasNoDuplicates(path + [onp])
+      && ONPValid(new_c, onp)
+      && (onp !in path)
+      && !PathExists(new_c, onp, Seq.Last(path))
+  {
+    var (new_c, new_s) := ConnectCircuitScufImpl(c, s, conn);
+    var onp: NP := new_c.PortSource[Seq.Last(path)];
+    conn.GetConnectionProperties(c, s);
+    var conn_outputs := conn.GetConnectedOutputs(s.mp);
+    var conn_inputs := conn.GetConnectedInputs(s.mp);
+    //assert PathValid(c, path) by {
+    //  assert PathValid(new_c, path);
+    //  reveal PathValid();
+    //}
+    assert ONPValid(new_c, onp) by {
+      reveal Circuit.Valid();
+    }
+    assert onp !in path by {
+      // We know there are no paths from onp to Seq.Last(path) because onp is one of the connected outputs,
+      // and Seq.Last(path) is one of the connected inputs, and we know there are no pathes between.
+      if onp in path {
+        var index := Seq.IndexOf(path, onp);
+        var path_contradict := ValidPathSegment(c, path, index, |path|);
+        assert PathFromTo(c, path_contradict, onp, Seq.Last(path));
+        assert onp in conn.GetConnectedOutputs(s.mp);
+        assert Seq.Last(path) in conn.GetConnectedInputs(s.mp);
+        assert PathBetweenNPSets(c, path_contradict, conn_outputs, conn_inputs);
+        reveal PathExistsBetweenNPSets();
+        assert PathExistsBetweenNPSets(c, conn_outputs, conn_inputs);
+      }
+    }
+    assert !PathExists(new_c, onp, Seq.Last(path)) by {
+      reveal PathExists();
+      reveal PathExistsBetweenNPSets();
+      NoPathExistsBetweenNPSetsToNoPathExists(new_c, conn_outputs, conn_inputs, onp, Seq.Last(path));
+    }
+    StillHasNoDuplicates(path, onp);
+    AppendPathValid(new_c, path, onp);
+  }
+
+
+  lemma EvaluateINPInnerSelfConnectHelperB(c: Circuit, s: Scuf, conn: InternalConnection, path: seq<NP>, fi: FI)
+    requires EvaluateINPInnerSelfConnectRequirements(c, s, conn, path, fi)
+    requires PathValid(c, path)
+    requires 
+      var fi_second_pass := conn.FISecondPass(s.mp, s.uf, fi);
+      && (Seq.Last(path) !in fi.inputs)
+      && (Seq.Last(path) in fi_second_pass.inputs)
+    ensures
+      var (new_c, new_s) := ConnectCircuitScufImpl(c, s, conn);
+      var onp: NP := new_c.PortSource[Seq.Last(path)];
+      var fi_first_pass := conn.FIFirstPass(s.mp, fi);
+      var conn_outputs := conn.GetConnectedOutputs(s.mp);
+      reveal FICircuitValid();
+      && PathValid(new_c, path + [onp])
+      && Seq.HasNoDuplicates(path + [onp])
+      && ONPValid(new_c, onp)
+      && (onp in conn_outputs)
+      && (EvaluateONPInner(new_c, path + [onp], fi) == EvaluateONPInner(new_c, path + [onp], fi_first_pass))
+  {
+    EvaluateINPInnerSelfConnectHelperA(c, s, conn, path, fi);
+    var (new_c, new_s) := ConnectCircuitScufImpl(c, s, conn);
+    var onp: NP := new_c.PortSource[Seq.Last(path)];
+    var fi_first_pass := conn.FIFirstPass(s.mp, fi);
+    conn.GetConnectionProperties(c, s);
+    EvaluateINPInnerSelfConnectHelperA(c, s, conn, path, fi);
+    var conn_outputs := conn.GetConnectedOutputs(s.mp);
+    var conn_inputs := conn.GetConnectedInputs(s.mp);
+    assert !PathExistsBetweenNPSets(new_c, conn_outputs, conn_inputs) by {
+      reveal ScufConnectionConsistent();
+      reveal ONPsValid();
+      StillNoPathExistsBetweenNPSets(c, new_c, conn_outputs, conn_inputs);
+    }
+    reveal FICircuitValid();
+    var output_width := |s.mp.outputs|;
+    var fake_output := seq(output_width, (index: nat) requires index < output_width => false);
+    assert Seq.Last(path) in conn_inputs;
+    assert onp in conn_outputs;
+    EvaluateONPInnerConnectedOutputs(c, s, conn, path + [onp], fi, fake_output);
+    assert EvaluateONPInner(new_c, path + [onp], fi) == EvaluateONPInner(new_c, path + [onp], fi_first_pass);
+  }
+
+
+  lemma EvaluateINPInnerSelfConnectHelper(c: Circuit, s: Scuf, conn: InternalConnection, path: seq<NP>, fi: FI)
+    requires EvaluateINPInnerSelfConnectRequirements(c, s, conn, path, fi)
+    requires PathValid(c, path)
+    requires 
+      var fi_second_pass := conn.FISecondPass(s.mp, s.uf, fi);
+      && (Seq.Last(path) !in fi.inputs)
+      && (Seq.Last(path) in fi_second_pass.inputs)
+    ensures
+      var (new_c, new_s) := ConnectCircuitScufImpl(c, s, conn);
+      var fi_second_pass := conn.FISecondPass(s.mp, s.uf, fi);
+      && (EvaluateINPInner(new_c, path, fi_second_pass) == EvaluateINPInner(new_c, path, fi))
+  {
+    var (new_c, new_s) := ConnectCircuitScufImpl(c, s, conn);
+    var head := Seq.Last(path);
+    var onp: NP := new_c.PortSource[head];
+    var output_width := |s.mp.outputs|;
+    var fake_output := seq(output_width, (index: nat) requires index < output_width => false);
+    var si_first_pass := conn.SIFromOutputs(s.mp, fi, fake_output);
+    var fi_first_pass := s.mp.si2fi(si_first_pass);
+    s.mp.si2fi2si(si_first_pass);
+    assert si_first_pass == conn.SIFromOutputs(s.mp, fi, fake_output);
+    assert s.uf.sf.requires(si_first_pass) by {
+      reveal UpdateFunction.Valid();
+    }
+    var so_first_pass := s.uf.sf(si_first_pass);
+    assert so_first_pass == conn.SOFirstPass(s.mp, s.uf, fi);
+    assert s.mp.so2fo.requires(so_first_pass) by {
+      reveal UpdateFunction.Valid();
+    }
+    var fo_first_pass := s.mp.so2fo(so_first_pass);
+    assert fo_first_pass == conn.FOFirstPass(s.mp, s.uf, fi);
+    var fi_second_pass := conn.FISecondPass(s.mp, s.uf, fi);
+    calc {
+      EvaluateINPInner(new_c, path, fi);
+      {
+        EvaluateINPInnerSelfConnectHelperA(c, s, conn, path, fi);
+      }
+      EvaluateONPInner(new_c, path + [onp], fi);
+      {
+        EvaluateINPInnerSelfConnectHelperB(c, s, conn, path, fi);
+        reveal FICircuitValid();
+      }
+      EvaluateONPInner(new_c, path + [onp], fi_first_pass);
+      {
+        var conn_outputs := conn.GetConnectedOutputs(s.mp);
+        assert onp in conn_outputs;
+        reveal Seq.ToSet();
+        assert onp in s.mp.outputs;
+        EvaluateINPInnerSelfConnectHelperA(c, s, conn, path, fi);
+        reveal PathValid();
+        EvaluateONPInnerConnectedOutputs(c, s, conn, path + [onp], fi, fake_output);
+      }
+      EvalOk(MFLookup(s, fi_first_pass, onp));
+      {
+        reveal Seq.ToSet();
+        EvaluateINPInnerSelfConnectHelperB(c, s, conn, path, fi);
+        assert onp in s.mp.outputs;
+      }
+      EvalOk(MFLookupOutput(s, fi_first_pass, onp));
+      EvalOk(fo_first_pass.outputs[onp]);
+      {
+        EvaluateINPInnerSelfConnectHelperB(c, s, conn, path, fi);
+        conn.FOFirstPassTOFISecondPass(s.mp, s.uf, fi, head);
+      }
+      EvalOk(fi_second_pass.inputs[head]);
+      EvaluateINPInner(new_c, path, fi_second_pass);
+    }
+    assert (EvaluateINPInner(new_c, path, fi_second_pass) == EvaluateINPInner(new_c, path, fi));
+  }
+
+  lemma {:vcs_split_on_every_assert} EvaluateINPInnerSelfConnect(c: Circuit, s: Scuf, conn: InternalConnection, path: seq<NP>, fi: FI)
+    requires c.Valid()
+    requires s.Valid(c)
+    requires conn.Valid()
+    requires ScufConnectionConsistent(c, s, conn)
+    //requires
+    //  reveal ScufConnectionConsistent();
+    //  forall np :: np in path ==> np !in conn.GetConnectedOutputs(s.mp)
+    requires
+      && var (new_c, new_s) := ConnectCircuitScufImpl(c, s, conn);
+      && FIValid(fi, new_s.mp.inputs, new_s.mp.state)
+      && var fi_second_pass := conn.FISecondPass(s.mp, s.uf, fi);
+      && EvaluateINPInnerRequirements(new_c, path, fi_second_pass)
+      && EvaluateINPInnerRequirements(new_c, path, fi)
+    ensures
+      var (new_c, new_s) := ConnectCircuitScufImpl(c, s, conn);
+      var fi_second_pass := conn.FISecondPass(s.mp, s.uf, fi);
+      && (EvaluateINPInner(new_c, path, fi_second_pass) == EvaluateINPInner(new_c, path, fi))
+    decreases
+      var (new_c, new_s) := ConnectCircuitScufImpl(c, s, conn);
+      |NodesNotInPath(new_c, path)|, 3
+  {
+    var (new_c, new_s) := ConnectCircuitScufImpl(c, s, conn);
+    var fi_first_pass := conn.FIFirstPass(s.mp, fi);
+    var so_first_pass := conn.SOFirstPass(s.mp, s.uf, fi);
+    var fi_second_pass := conn.FISecondPass(s.mp, s.uf, fi);
+    var head := path[|path|-1];
+    var tail := path[..|path|-1];
+    var connections := conn.GetConnection(s.mp);
+    if head in fi.inputs {
+      assert head in fi.inputs;
+      assert head in fi_second_pass.inputs;
+      conn.FISecondPassMatchingKeyMatchingValue(s.mp, s.uf, fi);
+      assert fi.inputs[head] == fi_second_pass.inputs[head];
+    } else if head in fi_second_pass.inputs {
+      assert head !in fi.inputs;
+      // We've gone from an onp to one of the connected inps;
+      // We need to prove that these two things are equal.
+      // EvaluateINPInner(new_c, path, fi_second_pass)
+      // EvaluateINPInner(new_c, path, fi))
+
+      // If fi_second_pass is used, then the value is just the value in fi_second_pass.
+      assert EvaluateINPInner(new_c, path, fi_second_pass) == EvalOk(fi_second_pass.inputs[head]);
+      // But if we're using 'fi' then  we propagate back to the connected onp.
+
+
+
+      assert head in s.mp.inputs &&  head !in new_s.mp.inputs by {
+        reveal Seq.ToSet();
+        assert head !in fi.inputs;
+        assert fi.inputs.Keys == Seq.ToSet(new_s.mp.inputs);
+      }
+      assert head in connections.Keys by {
+        reveal Seq.ToSet();
+        assert new_s.mp == ConnectScufMap(s.mp, conn);
+      }
+      var onp: NP := new_c.PortSource[head];
+      //assert head !in c.PortSource;
+      assert onp !in path by {
+        // We know there are no paths from onp to Seq.Last(path) because onp is one of the connected outputs,
+        // and Seq.Last(path) is one of the connected inputs, and we know there are no pathes between.
+        if onp in path {
+          var index := Seq.IndexOf(path, onp);
+          var path_contradict := ValidPathSegment(c, path, index, |path|);
+          assert PathFromTo(c, path_contradict, onp, Seq.Last(path));
+        }
+      }
+      // Prove has no duplicates
+      StillHasNoDuplicates(path, onp);
+      assert EvaluateINPInner(new_c, path, fi) == EvaluateONPInner(new_c, path + [onp], fi);
+       
+      //assert head in Seq.ToSet(s.mp.inputs);
+      //assert head in connections.Keys;
+      assert head !in c.PortSource by {
+        reveal ScufConnectionConsistent();
+      }
+      assert onp !in path;
+      reveal Circuit.Valid();
+      NodesNotInPathDecreases(new_c, path, onp);
+      StillHasNoDuplicates(path, onp);
+      AppendPathValid(new_c, path, onp);
+      // Look back around to ONP.
+      var connection := conn.GetConnection(s.mp); 
+      assert onp == connection[head];
+      assert ONPValid(new_c, onp);
+      assert EvaluateONPInnerRequirements(new_c, path + [onp], fi) by {
+          assert EvaluateConstRequirements(new_c, fi);
+          assert EvaluatePathRequirements(new_c, path + [onp]);
+          assert ONPValid(new_c, Seq.Last(path + [onp]));
+      }
+      assert EvaluateONPInnerRequirements(new_c, path + [onp], fi_second_pass);
+      assert FICircuitValid(new_c, fi);
+      assert FICircuitValid(new_c, fi_second_pass) && FICircuitValid(new_c, fi_first_pass) by {
+        reveal FICircuitValid();
+      }
+      var output_width := |s.mp.outputs|;
+      var fake_output := seq(output_width, (index: nat) requires index < output_width => false);
+      var sni := new_s.mp.fi2si(fi);
+      var si_second_pass_inputs := conn.NIO2I(sni.inputs, so_first_pass.outputs);
+      var si_second_pass := SI(si_second_pass_inputs, sni.state);
+      assert fi_second_pass == s.mp.si2fi(si_second_pass);
+
+      var actual_output := so_first_pass.outputs;
+      assert |actual_output| == |s.mp.outputs| by {
+        assert ScufMapUpdateFunctionConsistent(s.mp, s.uf);
+        assert s.uf.output_width == |s.mp.outputs|;
+        reveal UpdateFunction.Valid();
+        assert|so_first_pass.outputs| == s.uf.output_width;
+      }
+      EvaluateONPInnerConnectedOutputs(c, s, conn, path + [onp], fi, fake_output);
+      EvaluateONPInnerConnectedOutputs(c, s, conn, path + [onp], fi, actual_output);
+      assert EvaluateONPInner(new_c, path + [onp], fi_first_pass) == EvaluateONPInner(new_c, path + [onp], fi);
+      assert EvaluateONPInner(new_c, path + [onp], fi_second_pass) == EvaluateONPInner(new_c, path + [onp], fi);
+  //if head in fi.inputs then
+  //  EvalOk(fi.inputs[head])
+  //else
+  //  if head in c.PortSource then
+  //    var onp := c.PortSource[head];
+  //    if onp in path then
+  //      EvalError({}, {path + [onp]})
+  //    else
+      calc {
+        EvaluateINPInner(new_c, path, fi);
+        EvaluateONPInner(new_c, path + [onp], fi);
+        EvaluateONPInner(new_c, path + [onp], fi_first_pass);
+        Evaluate(new_c, onp, fi_first_pass);
+        EvalOk(MFLookup(s, fi_first_pass, onp));
+        //EvalOk(fo_first_pass.outputs[onp]);
+        EvalOk(fi_second_pass.inputs[head]);
+        EvaluateINPInner(new_c, path, fi_second_pass);
+      }
+      assert EvaluateINPInner(new_c, path, fi_second_pass) == EvaluateINPInner(new_c, path, fi);
+
+    } else if head in new_c.PortSource {
+      assert head !in Seq.ToSet(new_s.mp.inputs);
+      assert fi.inputs.Keys == Seq.ToSet(new_s.mp.inputs);
+      assert Seq.ToSet(new_s.mp.inputs) == Seq.ToSet(s.mp.inputs) - connections.Keys;
+      var onp: NP := new_c.PortSource[head];
+      if head in fi_second_pass.inputs {
+      } else {
+        reveal Circuit.Valid();
+        NodesNotInPathDecreases(new_c, path, onp);
+        StillHasNoDuplicates(path, onp);
+        AppendPathValid(new_c, path, onp);
+        EvaluateONPInnerSelfConnect(c, s, conn, path + [onp], fi);
+      }
+      assert SubcircuitWeaklyConserved(c, new_c, s.sc);
+      assert new_c.PortSource[head] == c.PortSource[head] by {
+        reveal SubcircuitWeaklyConserved();
+      }
+    } else {
+      //EvalError({head}, {})
+    }
+  }
+
+  lemma EvaluateONPUnarySelfConnect(c: Circuit, s: Scuf, conn: InternalConnection, path: seq<NP>, fi: FI)
+    requires c.Valid()
+    requires s.Valid(c)
+    requires conn.Valid()
+    requires ScufConnectionConsistent(c, s, conn)
+    requires
+      && var (new_c, new_s) := ConnectCircuitScufImpl(c, s, conn);
+      && FIValid(fi, new_s.mp.inputs, new_s.mp.state)
+      && var fi_second_pass := conn.FISecondPass(s.mp, s.uf, fi);
+      && EvaluateONPUnaryRequirements(new_c, path, fi_second_pass)
+      && EvaluateONPUnaryRequirements(new_c, path, fi)
+    ensures
+      var (new_c, new_s) := ConnectCircuitScufImpl(c, s, conn);
+      var fi_second_pass := conn.FISecondPass(s.mp, s.uf, fi);
+      && (EvaluateONPUnary(new_c, path, fi_second_pass) == EvaluateONPUnary(new_c, path, fi))
+    decreases
+      var (new_c, new_s) := ConnectCircuitScufImpl(c, s, conn);
+      |NodesNotInPath(new_c, path)|, 3
+  {
+    var (new_c, new_s) := ConnectCircuitScufImpl(c, s, conn);
+    var head := Seq.Last(path);
+    var nk := c.NodeKind[head.n];
+    assert nk == new_c.NodeKind[head.n];
+    assert NodeValid(c, head.n);
+    var inp_0 := NP(head.n, INPUT_0);
+    if inp_0 in path {
+    } else {
+      NodesNotInPathDecreases(new_c, path, inp_0);
+      var new_path_0 := path + [inp_0];
+      assert PathValid(new_c, new_path_0);
+      assert |NodesNotInPath(new_c, path + [inp_0])| < |NodesNotInPath(new_c, path)|;
+      StillHasNoDuplicates(path, inp_0);
+      EvaluateINPInnerSelfConnect(c, s, conn, path + [inp_0], fi);
+    }
+  }
+
+  lemma EvaluateONPBinarySelfConnect(c: Circuit, s: Scuf, conn: InternalConnection, path: seq<NP>, fi: FI)
+    requires c.Valid()
+    requires s.Valid(c)
+    requires conn.Valid()
+    requires ScufConnectionConsistent(c, s, conn)
+    requires
+      && var (new_c, new_s) := ConnectCircuitScufImpl(c, s, conn);
+      && FIValid(fi, new_s.mp.inputs, new_s.mp.state)
+      && var fi_second_pass := conn.FISecondPass(s.mp, s.uf, fi);
+      && EvaluateONPBinaryRequirements(new_c, path, fi_second_pass)
+      && EvaluateONPBinaryRequirements(new_c, path, fi)
+    ensures
+      var (new_c, new_s) := ConnectCircuitScufImpl(c, s, conn);
+      var fi_second_pass := conn.FISecondPass(s.mp, s.uf, fi);
+      && (EvaluateONPBinary(new_c, path, fi_second_pass) == EvaluateONPBinary(new_c, path, fi))
+    decreases
+      var (new_c, new_s) := ConnectCircuitScufImpl(c, s, conn);
+      |NodesNotInPath(new_c, path)|, 3
+  {
+    var (new_c, new_s) := ConnectCircuitScufImpl(c, s, conn);
+    var head := Seq.Last(path);
+    var nk := c.NodeKind[head.n];
+    assert nk == new_c.NodeKind[head.n];
+    assert NodeValid(c, head.n);
+    var inp_0 := NP(head.n, INPUT_0);
+    var inp_1 := NP(head.n, INPUT_1);
+    if inp_0 in path {
+    } else if inp_1 in path {
+    } else {
+      NodesNotInPathDecreases(new_c, path, inp_0);
+      NodesNotInPathDecreases(new_c, path, inp_1);
+      var new_path_0 := path + [inp_0];
+      var new_path_1 := path + [inp_1];
+      assert PathValid(new_c, new_path_0);
+      assert PathValid(new_c, new_path_1);
+      assert |NodesNotInPath(new_c, path + [inp_0])| < |NodesNotInPath(new_c, path)|;
+      StillHasNoDuplicates(path, inp_0);
+      StillHasNoDuplicates(path, inp_1);
+      EvaluateINPInnerSelfConnect(c, s, conn, path + [inp_0], fi);
+      EvaluateINPInnerSelfConnect(c, s, conn, path + [inp_1], fi);
+    }
+  }
+
+  lemma EvaluateONPInnerSelfConnect(c: Circuit, s: Scuf, conn: InternalConnection, path: seq<NP>, fi: FI)
+    requires c.Valid()
+    requires s.Valid(c)
+    requires conn.Valid()
+    requires ScufConnectionConsistent(c, s, conn)
+    requires
+      && var (new_c, new_s) := ConnectCircuitScufImpl(c, s, conn);
+      && FIValid(fi, new_s.mp.inputs, new_s.mp.state)
+      && var fi_second_pass := conn.FISecondPass(s.mp, s.uf, fi);
+      && EvaluateONPInnerRequirements(new_c, path, fi_second_pass)
+      && EvaluateONPInnerRequirements(new_c, path, fi)
+    ensures
+      var (new_c, new_s) := ConnectCircuitScufImpl(c, s, conn);
+      var fi_second_pass := conn.FISecondPass(s.mp, s.uf, fi);
+      && (EvaluateONPInner(new_c, path, fi_second_pass) == EvaluateONPInner(new_c, path, fi))
+    decreases
+      var (new_c, new_s) := ConnectCircuitScufImpl(c, s, conn);
+      |NodesNotInPath(new_c, path)|, 4
+  {
+    var (new_c, new_s) := ConnectCircuitScufImpl(c, s, conn);
+    var fi_second_pass := conn.FISecondPass(s.mp, s.uf, fi);
+    var head := path[|path|-1];
+    var nk := c.NodeKind[head.n];
+    assert nk == new_c.NodeKind[head.n];
+    if head.n in fi.state {
+      assert nk.CSeq? by {
+        reveal FICircuitValid();
+      }
+      match nk
+        case CSeq() => {
+          assert fi.state[head.n] == fi_second_pass.state[head.n];
+        }
+    } else {
+      match nk
+        case CXor() => {
+            EvaluateONPBinarySelfConnect(c, s, conn, path, fi);
+        }
+        case CAnd() => {
+            EvaluateONPBinarySelfConnect(c, s, conn, path, fi);
+        }
+        case CInv() => {
+            EvaluateONPUnarySelfConnect(c, s, conn, path, fi);
+        }
+        case CIden() => {
+            EvaluateONPUnarySelfConnect(c, s, conn, path, fi);
+        }
+        case CConst(b) => {
+        }
+        case CSeq() => {
+        }
+    }
+  }
+
+  //lemma EvaluateONP(c: Circuit, s: Scuf, conn: InternalConnection, np: NP, fi: FI)
+  //  //
+  //  // Here we need to prove that when we take a circuit and connect some of the input points to
+  //  // other nodes it doesn't effect the evaluation.
+  //  // This is because at the input points the evaluation is terminated.
+  //  //
+  //  //
+  //  requires c.Valid()
+  //  requires s.Valid(c)
+  //  requires conn.Valid()
+  //  requires ScufConnectionConsistent(c, s, conn)
+  //  requires FIValid(fi, s.mp.inputs, s.mp.state)
+  //  requires NPValid(c, np)
+  //  requires np in s.mp.outputs || np in StateINPs(s.mp.state)
+  //  ensures
+  //    var (new_c, new_s) := ConnectCircuitScufImpl(c, s, conn);
+  //    && FICircuitValid(new_c, fi)
+  //    && FICircuitValid(c, fi)
+  //    && (Evaluate(new_c, np, fi) == Evaluate(c, np, fi))
+  //{
+  //}
+}
